cedar-lean/Cedar/Thm/BatchedEvaluator/Common.lean
@@ -1,0 +1,86 @@
+import Cedar.TPE.Input
+import Cedar.TPE.BatchedEvaluator
+import Cedar.Spec
+import Cedar.Thm.TPE.Input
+
+/-!
+Shared definitions and lemmas for batched evaluator theorems.
+-/
+
+namespace Cedar.Thm
+
+open Cedar.TPE
+open Cedar.Spec
+open Cedar.Data
+
+/-- A well behaved entity loader
+1. Loads all the requested entities, returning none for missing
+entities
+2. Refines the backing entity store
+
+The first condition is required for convergence of
+batched evaluation, which has not been proven. It is unused
+in the code base at the moment.
+-/
+abbrev EntityLoader.WellBehaved (store: Entities) (loader: EntityLoader) : Prop :=
+  ∀ s, s ⊆ (loader s).keys ∧
+       EntitiesRefine store ((loader s).mapOnValues MaybeEntityData.asPartial)
+
+theorem as_partial_request_refines {req : Request} :
+  RequestRefines req req.asPartialRequest := by
+  simp only [Request.asPartialRequest, RequestRefines, PartialEntityUID.asEntityUID, Option.map_some]
+  constructor
+  · apply PartialIsValid.some
+    rfl
+  constructor
+  · trivial
+  constructor
+  · apply PartialIsValid.some
+    rfl
+  constructor
+  · apply PartialIsValid.some
+    rfl
+  constructor <;> trivial
+
+theorem any_refines_empty_entities :
+  EntitiesRefine es Data.Map.empty := by
+  simp only [EntitiesRefine, Data.Map.empty, Data.Map.find?, Map.toList]
+  intro a e₂ h₁
+  contradiction
+
+theorem entities_refine_append (es : Entities) (m1 m2 : PartialEntities) :
+  EntitiesRefine es m1 → EntitiesRefine es m2 → EntitiesRefine es (m2 ++ m1) := by
+  intro h1 h2
+  unfold EntitiesRefine
+  intro a e₂ h_find
+  rw [Map.find?_append] at h_find
+  cases h_case : m2.find? a with
+  | some e₂' =>
+    have h_eq : e₂ = e₂' := by
+      rw [h_case] at h_find
+      simp only [Option.some_or, Option.some.injEq] at h_find
+      rw [h_find]
+    rw [h_eq]
+    exact h2 a e₂' h_case
+  | none =>
+    have h_find1 : m1.find? a = some e₂ := by
+      rw [h_case] at h_find
+      simp only [Option.none_or] at h_find
+      rw [h_find]
+    exact h1 a e₂ h_find1
+
+theorem direct_request_and_entities_refine (req : Request) (es : Entities) :
+  RequestAndEntitiesRefine req es req.asPartialRequest es.asPartial := by
+  constructor
+  · exact as_partial_request_refines
+  · unfold EntitiesRefine Entities.asPartial
+    intro uid data₂ h_find
+    have h_mapOnValues := Map.find?_mapOnValues_some' EntityData.asPartial h_find
+    obtain ⟨data₁, h_find₁, h_eq⟩ := h_mapOnValues
+    exists data₁
+    exact ⟨h_find₁,
+           by rw [h_eq]; apply PartialIsValid.some; rfl,
+           by rw [h_eq]; apply PartialIsValid.some; rfl,
+           by rw [h_eq]; apply PartialIsValid.some; rfl⟩
+
+end Cedar.Thm
